src/QueryStructure/Refinements/Bags/BagsOfTuples.v
@@ -34,98 +34,318 @@ Module ZTreeBag := TreeBag ZIndexedMap.
 Module NatTreeBag := TreeBag NatIndexedMap.
 Module StringTreeBag := TreeBag StringIndexedMap.
 
-Definition TTreeConstructor (TKey: Type) :=
-  forall TBag TItem TBagSearchTerm TBagUpdateTerm : Type,
-  Bag TBag TItem TBagSearchTerm TBagUpdateTerm
-  -> (TItem -> TKey) -> Type.
+Definition NTreeType      := @NTreeBag.IndexedBag.
+Definition ZTreeType      := @ZTreeBag.IndexedBag.
+Definition NatTreeType    := @NatTreeBag.IndexedBag.
+Definition StringTreeType := @StringTreeBag.IndexedBag.
 
-Definition mkTreeType
-           (TKey: Type)
-           (tree_constructor: TTreeConstructor TKey)
-           TSubtree TSubtreeSearchTerm TSubtreeUpdateTerm
-           heading projection subtree_as_bag : Type :=
-  tree_constructor TSubtree (@Tuple heading) TSubtreeSearchTerm
-                   TSubtreeUpdateTerm projection subtree_as_bag.
+Record ProperAttribute {heading} :=
+  {
+    Attribute : Attributes heading;
+    ProperlyTyped: { Domain heading Attribute = BinNums.N } + { Domain heading Attribute = BinNums.Z } +
+                   { Domain heading Attribute = nat } + { Domain heading Attribute = string }
+  }.
 
-Definition NTreeType      := mkTreeType BinNums.N (@NTreeBag.IndexedBag).
-Definition ZTreeType      := mkTreeType BinNums.Z (@ZTreeBag.IndexedBag).
-Definition NatTreeType    := mkTreeType nat       (@NatTreeBag.IndexedBag).
-Definition StringTreeType := mkTreeType string    (@StringTreeBag.IndexedBag).
+Definition ProperAttributeToFMap
+           {heading}
+           (pattr : @ProperAttribute heading)
+: Type -> Type :=
+  let (attr', cast) := pattr in
+  match cast with
+    | inleft (inleft (left cast'))  => @NTreeBag.IndexedBag
+    | inleft (inleft (right cast')) => @ZTreeBag.IndexedBag
+    | inleft (inright cast')         => @NatTreeBag.IndexedBag
+    | inright cast'                  => @StringTreeBag.IndexedBag
+  end.
+
+Fixpoint NestedTreeFromAttributes
+         {heading}
+         (indices : list (@ProperAttribute heading))
+: Type :=
+  match indices with
+    | [] => @CountingList (@Tuple heading)
+    | idx :: indices' =>
+      ProperAttributeToFMap idx (NestedTreeFromAttributes indices')
+  end.
+
+Definition ProperAttributeToFMapKey
+           {heading}
+           (pattr : @ProperAttribute heading)
+: Type :=
+  let (attr', cast) := pattr in
+  match cast with
+    | inleft (inleft (left cast'))  => @NTreeBag.TKey
+    | inleft (inleft (right cast')) => @ZTreeBag.TKey
+    | inleft (inright cast')         => @NatTreeBag.TKey
+    | inright cast'                  => @StringTreeBag.TKey
+  end.
+
+Fixpoint BuildSearchTermFromAttributes {heading}
+         (indices : list (@ProperAttribute heading))
+: Type :=
+  match indices with
+      | [] => (list (@Tuple heading -> bool))
+      | idx :: indices' => prod (option (ProperAttributeToFMapKey idx)) (BuildSearchTermFromAttributes indices')
+  end.
 
 Definition cast {T1 T2: Type} (eq: T1 = T2) (x: T1) : T2.
 Proof.
   subst; auto.
 Defined.
 
-Record ProperAttribute {heading} :=
-  {
-    Attribute :> Attributes heading;
-    ProperlyTyped: { Domain heading Attribute = BinNums.N } + { Domain heading Attribute = BinNums.Z } +
-                   { Domain heading Attribute = nat } + { Domain heading Attribute = string }
-  }.
+Definition ProperAttributeToBag
+           {heading}
+           TBag TSearchTerm TUpdateTerm
+           (TBagAsBag : Bag TBag (@Tuple heading) TSearchTerm TUpdateTerm)
+           (pattr : @ProperAttribute heading)
+: Bag (ProperAttributeToFMap pattr TBag) (@Tuple heading)
+      (prod (option (ProperAttributeToFMapKey pattr)) TSearchTerm) TUpdateTerm :=
+  match pattr as pattr' return
+        Bag (ProperAttributeToFMap pattr' TBag) (@Tuple heading)
+            (prod (option (ProperAttributeToFMapKey pattr')) TSearchTerm) TUpdateTerm with
+    | {| Attribute := attr; ProperlyTyped := inleft (inleft (left cast')) |}
+      => NTreeBag.IndexedBagAsBag TBagAsBag (fun x => cast cast' (x attr))
+    | {| Attribute := attr; ProperlyTyped := inleft (inleft (right cast')) |}
+      => ZTreeBag.IndexedBagAsBag TBagAsBag (fun x => cast cast' (x attr))
+    | {| Attribute := attr; ProperlyTyped := inleft (inright cast') |}
+      => NatTreeBag.IndexedBagAsBag TBagAsBag (fun x => cast cast' (x attr))
+    | {| Attribute := attr; ProperlyTyped := inright cast' |}
+      => StringTreeBag.IndexedBagAsBag TBagAsBag (fun x => cast cast' (x attr))
+  end.
 
-Record KeyPreservingUpdateF {heading}
-       (indices : list (@ProperAttribute heading))
-  :=
-  { KPUpdate_F : @Tuple heading -> @Tuple heading;
-    ValidUpdate_F :
-      forall K tup,
-        In K indices
-        -> KPUpdate_F tup (@Attribute _ K) = tup (@Attribute _ K)}.
-
-Instance TupleListAsBag
-         (heading: Heading)
-         indices
-: Bag (@CountingList (@Tuple heading)) (@Tuple heading)
-      (list (TSearchTermMatcher heading))
-      (@KeyPreservingUpdateF heading indices).
-Proof.
-  apply CountingListAsBag.
-  econstructor 1 with (KPUpdate_F := @id _); reflexivity.
-  intro KP; apply (KPUpdate_F _ KP).
-Defined.
-
-Definition foo 
+ Fixpoint NestedTreeFromAttributesAsBag
          heading
-         (Keys : list (@ProperAttribute heading))
-  := 
-    {| BagType        := @CountingList (@Tuple heading);
-       SearchTermType := list (TSearchTermMatcher heading);
-       BagProof       := TupleListAsBag heading Keys |}.
-
-Program Fixpoint NestedTreeFromAttributes'
-         heading
+         TUpdateTerm
+         (bid : TUpdateTerm)
+         (bupdate_transform : TUpdateTerm -> @Tuple heading -> @Tuple heading)
          (indices : list (@ProperAttribute heading))
-         (Keys : list (@ProperAttribute heading))
-         {struct indices}
-: @BagPlusBagProof (@Tuple heading) (@KeyPreservingUpdateF heading Keys) :=
-  match indices with
-    | [] => foo heading Keys
-    | proper_attr :: more_indexes =>  
-      let attr := @Attribute heading proper_attr in
-      let (t, st, bagproof) := NestedTreeFromAttributes' heading more_indexes Keys in
-      match @ProperlyTyped _ proper_attr with
-        | inleft (inleft (left conv))  =>
-          {| BagType        := NTreeType t st _ heading bagproof (fun x => cast conv (x attr));
-             SearchTermType := option BinNums.N * st;
-             BagProof := NTreeBag.IndexedBagAsBag 
-                           (NestedTreeFromAttributes' heading more_indexes Keys)
-                           (fun x => cast conv (x attr))
-          |}
-        | _ => _ end
+: Bag (NestedTreeFromAttributes indices)
+      (@Tuple heading)
+      (BuildSearchTermFromAttributes indices)
+      TUpdateTerm :=
+   match indices return 
+         Bag (NestedTreeFromAttributes indices)
+             (@Tuple heading)
+             (BuildSearchTermFromAttributes indices)
+               TUpdateTerm with
+     | [] => CountingListAsBag bid bupdate_transform
+     | idx :: indices' => ProperAttributeToBag 
+                            _ _ _ 
+                            (NestedTreeFromAttributesAsBag heading _ bid bupdate_transform indices') idx
+   end.
+
+Definition ProperAttributeToRepInv
+           {heading}
+           TBag TSearchTerm TUpdateTerm
+           (RepInv : TBag -> Prop)
+           (TBagAsBag : Bag TBag (@Tuple heading) TSearchTerm TUpdateTerm)
+           (pattr : @ProperAttribute heading)
+: (@Tuple heading -> ProperAttributeToFMapKey pattr)
+  -> ProperAttributeToFMap pattr TBag -> Prop  :=
+  match pattr as pattr' return 
+        (@Tuple heading -> ProperAttributeToFMapKey pattr')
+        -> ProperAttributeToFMap pattr' TBag -> Prop with
+    | {| Attribute := attr; ProperlyTyped := inleft (inleft (left cast')) |}
+      => NTreeBag.IndexedBag_RepInv TBagAsBag RepInv
+    | {| Attribute := attr; ProperlyTyped := inleft (inleft (right cast')) |}
+      => ZTreeBag.IndexedBag_RepInv TBagAsBag RepInv
+    | {| Attribute := attr; ProperlyTyped := inleft (inright cast') |}
+      => NatTreeBag.IndexedBag_RepInv TBagAsBag RepInv 
+    | {| Attribute := attr; ProperlyTyped := inright cast' |}
+      => StringTreeBag.IndexedBag_RepInv TBagAsBag RepInv 
   end.
 
-        | inleft (inleft (right conv)) =>
-          {| BagType        := ZTreeType t st upt heading bagproof (fun x => cast conv (x attr));
-             SearchTermType := option BinNums.Z * st |}
-        | inleft (inright conv)        =>
-          {| BagType        := NatTreeType t st upt heading bagproof (fun x => cast conv (x attr));
-             SearchTermType := option nat * st |}
-        | inright conv                 =>
-          {| BagType        := StringTreeType t st upt heading bagproof (fun x => cast conv (x attr));
-             SearchTermType := option string * st |}
-      end
+Definition ProperAttributeToProjection 
+           {heading}
+           (pattr : @ProperAttribute heading)
+: @Tuple heading -> ProperAttributeToFMapKey pattr :=
+  match pattr as pattr' return
+        @Tuple heading -> ProperAttributeToFMapKey pattr' with
+    | {| Attribute := attr; ProperlyTyped := inleft (inleft (left cast')) |}
+      => fun x => cast cast' (x attr)
+    | {| Attribute := attr; ProperlyTyped := inleft (inleft (right cast')) |}
+      => fun x => cast cast' (x attr)
+    | {| Attribute := attr; ProperlyTyped := inleft (inright cast') |}
+      => fun x => cast cast' (x attr)
+    | {| Attribute := attr; ProperlyTyped := inright cast' |}
+      => fun x => cast cast' (x attr)
   end.
+
+Definition ProperAttributeToValidUpdate
+           {heading}
+           TBag TSearchTerm TUpdateTerm
+           (ValidUpdate : TUpdateTerm -> Prop)
+           (TBagAsBag : Bag TBag (@Tuple heading) TSearchTerm TUpdateTerm)
+           (pattr : @ProperAttribute heading)
+: (@Tuple heading -> ProperAttributeToFMapKey pattr)
+  -> TUpdateTerm -> Prop  :=
+  match pattr as pattr' return 
+        (@Tuple heading -> ProperAttributeToFMapKey pattr')
+        -> TUpdateTerm -> Prop with
+    | {| Attribute := attr; ProperlyTyped := inleft (inleft (left cast')) |}
+      => NTreeBag.IndexedBag_ValidUpdate TBagAsBag ValidUpdate
+    | {| Attribute := attr; ProperlyTyped := inleft (inleft (right cast')) |}
+      => ZTreeBag.IndexedBag_ValidUpdate TBagAsBag ValidUpdate
+    | {| Attribute := attr; ProperlyTyped := inleft (inright cast') |}
+      => NatTreeBag.IndexedBag_ValidUpdate TBagAsBag ValidUpdate 
+    | {| Attribute := attr; ProperlyTyped := inright cast' |}
+      => StringTreeBag.IndexedBag_ValidUpdate TBagAsBag ValidUpdate 
+  end.
+
+ Definition ProperAttributeToCorrectBag
+           {heading}
+           TBag TSearchTerm TUpdateTerm
+           (TBagAsBag : Bag TBag (@Tuple heading) TSearchTerm TUpdateTerm)
+           (RepInv : TBag -> Prop)
+           (ValidUpdate : TUpdateTerm -> Prop)
+           (TBagAsCorrectBag : CorrectBag RepInv ValidUpdate TBagAsBag)
+           (pattr : @ProperAttribute heading)
+ :  CorrectBag (ProperAttributeToRepInv _ _ _ RepInv TBagAsBag pattr 
+                                         (ProperAttributeToProjection pattr)) 
+               (ProperAttributeToValidUpdate  _ _ _ ValidUpdate TBagAsBag pattr
+                                              (ProperAttributeToProjection pattr)) 
+               (ProperAttributeToBag TBag TSearchTerm TUpdateTerm TBagAsBag pattr) :=
+  match pattr as pattr' return 
+        CorrectBag (ProperAttributeToRepInv _ _ _ RepInv TBagAsBag pattr' 
+                                            (ProperAttributeToProjection pattr')) 
+               (ProperAttributeToValidUpdate  _ _ _ ValidUpdate TBagAsBag pattr'
+                                              (ProperAttributeToProjection pattr')) 
+                   (ProperAttributeToBag TBag TSearchTerm TUpdateTerm TBagAsBag pattr') with
+    | {| Attribute := attr; ProperlyTyped := inleft (inleft (left cast')) |}
+      => NTreeBag.IndexedBagAsCorrectBag TBagAsBag RepInv ValidUpdate TBagAsCorrectBag 
+                                         (fun x => cast cast' (x attr))
+    | {| Attribute := attr; ProperlyTyped := inleft (inleft (right cast')) |}
+      => ZTreeBag.IndexedBagAsCorrectBag TBagAsBag RepInv ValidUpdate TBagAsCorrectBag 
+                                         (fun x => cast cast' (x attr))
+    | {| Attribute := attr; ProperlyTyped := inleft (inright cast') |}
+      => NatTreeBag.IndexedBagAsCorrectBag TBagAsBag RepInv ValidUpdate TBagAsCorrectBag 
+                                         (fun x => cast cast' (x attr))
+    | {| Attribute := attr; ProperlyTyped := inright cast' |}
+      => StringTreeBag.IndexedBagAsCorrectBag TBagAsBag RepInv ValidUpdate TBagAsCorrectBag 
+                                         (fun x => cast cast' (x attr))
+  end.
+
+ Fixpoint ProperAttributesToRepInv
+          {heading}
+          TUpdateTerm
+          (bid : TUpdateTerm)
+          (bupdate_transform : TUpdateTerm -> @Tuple heading -> @Tuple heading)
+          (indices : list (@ProperAttribute heading))
+ : NestedTreeFromAttributes indices -> Prop :=
+   match indices return NestedTreeFromAttributes indices -> Prop with
+     | [] => CountingList_RepInv
+     | idx :: indices' => 
+       ProperAttributeToRepInv _ _ TUpdateTerm
+         (ProperAttributesToRepInv TUpdateTerm bid bupdate_transform indices')
+         (NestedTreeFromAttributesAsBag heading TUpdateTerm bid bupdate_transform indices') idx
+         (ProperAttributeToProjection idx)
+   end.
+
+ Fixpoint ProperAttributesToValidUpdate
+          {heading}
+          TUpdateTerm
+          (bid : TUpdateTerm)
+          (bupdate_transform : TUpdateTerm -> @Tuple heading -> @Tuple heading)
+          (indices : list (@ProperAttribute heading))
+ : TUpdateTerm -> Prop :=
+   match indices return TUpdateTerm -> Prop with
+     | [] => CountingList_ValidUpdate
+     | idx :: indices' => 
+       ProperAttributeToValidUpdate _ _ TUpdateTerm
+         (ProperAttributesToValidUpdate TUpdateTerm bid bupdate_transform indices')
+         (NestedTreeFromAttributesAsBag heading TUpdateTerm bid bupdate_transform indices') idx
+         (ProperAttributeToProjection idx)
+   end.
+
+ Program Fixpoint NestedTreeFromAttributesAsCorrectBag
+         heading
+         TUpdateTerm
+         (bid : TUpdateTerm)
+         (bupdate_transform : TUpdateTerm -> @Tuple heading -> @Tuple heading)
+         (indices : list (@ProperAttribute heading))
+ : CorrectBag (ProperAttributesToRepInv TUpdateTerm bid bupdate_transform indices)
+              (ProperAttributesToValidUpdate TUpdateTerm bid bupdate_transform indices)
+              (NestedTreeFromAttributesAsBag heading TUpdateTerm
+                                             bid bupdate_transform indices) :=
+   match indices return 
+         CorrectBag (ProperAttributesToRepInv TUpdateTerm bid bupdate_transform indices)
+                    (ProperAttributesToValidUpdate TUpdateTerm bid bupdate_transform indices)
+                    (NestedTreeFromAttributesAsBag heading TUpdateTerm
+                                   bid bupdate_transform indices) with
+     | [] => CountingListAsCorrectBag bid bupdate_transform
+     | idx :: indices' => 
+       ProperAttributeToCorrectBag
+         _ _ _ 
+         (NestedTreeFromAttributesAsBag heading TUpdateTerm bid bupdate_transform indices')
+         (ProperAttributesToRepInv TUpdateTerm bid bupdate_transform indices')
+         (ProperAttributesToValidUpdate TUpdateTerm bid bupdate_transform indices')
+         (NestedTreeFromAttributesAsCorrectBag heading TUpdateTerm bid bupdate_transform
+                                                 indices')
+           idx
+   end.
+
+Lemma bupdate_transform_NestedTree : 
+  forall heading
+         TUpdateTerm
+         (bid : TUpdateTerm)
+         (bupdate_transform' : TUpdateTerm -> @Tuple heading -> @Tuple heading)
+         (indices : list (@ProperAttribute heading)),
+    bupdate_transform
+      (Bag := NestedTreeFromAttributesAsBag _ _ bid bupdate_transform' indices) = 
+    bupdate_transform'.
+Proof.
+  induction indices; simpl; eauto.
+  destruct a as [attr [[[s | s] | s] | s ]]; simpl in *; eauto.
+Qed.
+
+Lemma KeyPreservingUpdateFAsUpdateTermOK {heading}
+: forall (indices indices' : list (@ProperAttribute heading))
+         (f : @Tuple heading -> @Tuple heading),
+    (forall a, List.In a indices -> List.In a indices')
+    -> (forall K tup, 
+          In K indices'
+          -> f tup (@Attribute _ K) = tup (@Attribute _ K))
+    -> ProperAttributesToValidUpdate (@Tuple heading -> @Tuple heading)
+                                     (id)
+                                     (fun upd tup => upd tup)
+                                     indices f.
+Proof.
+  induction indices; simpl; intuition.
+  - unfold CountingList_ValidUpdate; auto.
+  - destruct a as [attr [[[s | s] | s] | s ]]; simpl in *.
+    + unfold NTreeBag.IndexedBag_ValidUpdate; intuition.
+      eapply (IHindices indices'); eauto.
+      rewrite bupdate_transform_NestedTree, <- H1.
+      erewrite (H0 {| Attribute := attr; ProperlyTyped := inleft (inleft in_left) |}); 
+        simpl; eauto.
+    + unfold ZTreeBag.IndexedBag_ValidUpdate; intuition.
+      eapply (IHindices indices'); eauto.
+      rewrite bupdate_transform_NestedTree, <- H1.
+      erewrite (H0 {| Attribute := attr; ProperlyTyped := inleft (inleft in_right) |}); 
+        simpl; eauto.
+    + unfold NatTreeBag.IndexedBag_ValidUpdate; intuition.
+      eapply (IHindices indices'); eauto.
+      rewrite bupdate_transform_NestedTree, <- H1.
+      erewrite (H0 {| Attribute := attr; ProperlyTyped := inleft (inright s) |}); 
+        simpl; eauto.
+    + unfold StringTreeBag.IndexedBag_ValidUpdate; intuition.
+      eapply (IHindices indices'); eauto.
+      rewrite bupdate_transform_NestedTree, <- H1.
+      erewrite (H0 {| Attribute := attr; ProperlyTyped := inright s |}); 
+        simpl; eauto.
+Qed.
+
+Definition NestedTreeFromAttributesAsCorrectBag_UpdateF
+          {heading}
+          (indices : list (@ProperAttribute heading))
+: CorrectBag (ProperAttributesToRepInv _ _ _ indices)
+             (ProperAttributesToValidUpdate _ _ _ indices)
+             (NestedTreeFromAttributesAsBag heading 
+                                            (@Tuple heading -> @Tuple heading)
+                                            id
+                                            (fun upd tup => upd tup)
+                                            indices)
+  := NestedTreeFromAttributesAsCorrectBag heading _ _ _ _.
 
 Definition CheckType {heading} (attr: Attributes heading) (rightT: _) :=
   {| Attribute := attr; ProperlyTyped := rightT |}.
@@ -144,26 +364,35 @@ Ltac autoconvert func :=
 Ltac mkIndex heading attributes :=
   set (src := attributes);
   assert (list (@ProperAttribute heading)) as decorated_source by autoconvert (@CheckType heading);
-  apply (NestedTreeFromAttributes' heading decorated_source).
+  apply (ProperAttributeToFMap heading decorated_source).
 
 Require Import QueryStructureNotations ListImplementation.
 Require Import AdditionalLemmas AdditionalPermutationLemmas Arith.
 
 Lemma bempty_correct_DB :
-  forall {TContainer TSearchTerm : Type} {db_schema : QueryStructureSchema}
-         {index : BoundedString} {store_is_bag : Bag TContainer Tuple TSearchTerm},
-    EnsembleIndexedListEquivalence
+  forall {TContainer TSearchTerm TUpdateTerm : Type} 
+         {db_schema : QueryStructureSchema}
+         {index : BoundedString} 
+         {store_is_bag : Bag TContainer Tuple TSearchTerm TUpdateTerm}
+         (RepInv : TContainer -> Prop)
+         (ValidUpdate : TUpdateTerm -> Prop),
+    CorrectBag RepInv ValidUpdate store_is_bag 
+    -> EnsembleIndexedListEquivalence
       (GetUnConstrRelation (DropQSConstraints (QSEmptySpec db_schema)) index)
       (benumerate bempty).
 Proof.
   intros.
-  rewrite benumerate_empty_eq_nil.
+  erewrite benumerate_empty_eq_nil by eauto.
   apply EnsembleIndexedListEquivalence_Empty.
 Qed.
 
-Lemma binsert_correct_DB {TContainer TSearchTerm} :
-  forall db_schema qs index (store: TContainer),
-  forall {store_is_bag: Bag TContainer _ TSearchTerm},
+Lemma binsert_correct_DB {TContainer TSearchTerm TUpdateTerm} 
+      (RepInv : TContainer -> Prop)
+      (ValidUpdate : TUpdateTerm -> Prop):
+  forall db_schema qs index (store: TContainer)
+         {store_is_bag: Bag TContainer _ TSearchTerm TUpdateTerm}
+         (bag_is_valid : CorrectBag RepInv ValidUpdate store_is_bag)
+         (store_is_valid : RepInv store),
     EnsembleIndexedListEquivalence
       (GetUnConstrRelation qs index)
       (benumerate (Bag := store_is_bag) store) ->
@@ -185,14 +414,14 @@ Proof.
   setoid_rewrite NoDup_modulo_permutation.
   split; intros.
 
-  rewrite binsert_enumerate_length;
+  erewrite binsert_enumerate_length by eauto;
     destruct H0; subst;
     [ | apply lt_S];
     intuition.
 
   destruct H as (indices & [ l' (map & nodup & equiv) ]).
 
-  destruct (permutation_map_cons indexedTuple (binsert_enumerate tuple store)
+  destruct (permutation_map_cons indexedTuple (binsert_enumerate tuple store store_is_valid)
                                  {| tupleIndex := Datatypes.length (benumerate store);
                                     indexedTuple := tuple |} l' eq_refl map)
     as [ l'0 (map' & perm) ].
@@ -212,10 +441,10 @@ Proof.
   setoid_rewrite eq_sym_iff at 1.
   reflexivity.
 Qed.
-
+(*
 Ltac binsert_correct_DB :=
   match goal with
     | [ H: EnsembleIndexedListEquivalence (GetUnConstrRelation ?qs ?index)
                                           (benumerate (Bag := ?bagproof) ?store) |- _ ] =>
       solve [ simpl; apply (binsert_correct_DB (store_is_bag := bagproof) _ qs index _ H) ]
-  end.
+  end. *)
